---
title: " DTOJ4064简单的函数\t\t"
tags:
  - 数论
url: 5562.html
id: 5562
categories:
  - Solution
date: 2018-12-16 15:27:27
---

Min_25筛模板题。 $f(p)=p-1,f(2)=3$，可以通过这两个算出$H(n)$。 其他具体做法可以见[积性函数求和理论](http://www.dtenomde.com/author=iftest614/article=5370/)

#include<bits/stdc++.h>
#define N 100005
#define mod 1000000007
#define inv2 500000004
#define ll long long 
int pri\[N\], pcnt, vis\[N\], t1\[N\], t2\[N\], cnt;
ll lst\[N << 1\], h\[N << 1\]\[2\], n, sum\[N\];
 
void init ()
{
    for (int i = 2; i < N; i++)
    {
        sum\[i\] = sum\[i - 1\];
        if (!vis\[i\]) pri\[++pcnt\] = i, sum\[i\] += i;
        for (int j = 1; j <= pcnt && i*pri\[j\] < N; j++)
        {
            vis\[i*pri\[j\]\] = 1;
            if (i%pri\[j\] == 0) break;
        }
    }
}
int mul (int x) { return x >= mod ? x - mod : x; }
ll Pow (ll x, ll k) { ll t = 1; for (; k; k >>= 1, x = x * x%mod) if (k & 1) t = t * x%mod; return t; }
ll Sum (ll x) { return x == 1 ? 1 : (x % mod * ((x + 1) % mod) % mod * inv2 % mod); }
ll H (ll x) { return x >= N ? h\[t2\[n / x\]\]\[0\] : h\[t1\[x\]\]\[0\]; }
ll g (ll n, ll m)
{
    if (n == 1 || pri\[m\] >= n) return 0;
    ll res = (H (n) - (sum\[pri\[m\]\] - m) + mod) % mod;
    if (1ll * pri\[m\] * pri\[m\] >= n) return res - 2;
    if (n) res -= 2;
    for (int i = m + 1; 1ll * pri\[i\] * pri\[i\] <= n; i++)
        for (ll pe = pri\[i\], e = 1; pe <= n; pe *= pri\[i\], e++)
            res = (res + (pri\[i\] ^ e)*((e > 1) + g (n / pe, i))) % mod;
    return res;
}
int main ()
{
    std::cin >> n; 
    //n = 9876543210;
    init ();
    for (ll i = 1, j; i <= n; i = j + 1)
    {
        j = n / (n / i); ll t = n / i;
        lst\[++cnt\] = t; h\[cnt\]\[0\] = (Sum (t) - 1) % mod, h\[cnt\]\[1\] = (t - 1) % mod;
        t >= N ? t2\[n / t\] = cnt : t1\[t\] = cnt;
    }
    for (int i = 1; i <= pcnt; i++) 
    {
        if (1ll * pri\[i\] * pri\[i\] > n) break;
        for (int j = 1; lst\[j\] >= 1ll * pri\[i\] * pri\[i\]; j++)
        {
            ll t = lst\[j\] / pri\[i\], id = t >= N ? t2\[n / t\] : t1\[t\];
            h\[j\]\[0\] = (h\[j\]\[0\] - 1ll * (h\[id\]\[0\] - sum\[pri\[i - 1\]\]) * pri\[i\] % mod) % mod;
            h\[j\]\[1\] = (h\[j\]\[1\] - (h\[id\]\[1\] - (i - 1)) % mod) % mod;
        }
    }
    for (int i = 1; i <= cnt; i++)
    {
        h\[i\]\[0\] -= h\[i\]\[1\];
        if (lst\[i\] > 1) h\[i\]\[0\] += 2;
    }
    std::cout << (g (n, 0) + (n > 1) * 2 + 1 + mod) % mod << "\\n";
}